templates/hindsight/hindsight_proof.v
@@ -13,34 +13,27 @@ Module Type HINDSIGHT_SPEC (DS : DATA_STRUCTURE).
   Module DEFS := HINDSIGHT_DEFS DS.
   Import DS DEFS.
 
-  Definition is_updating (pvs : list (val * val)) : Prop :=
-    Exists (λ x, ∃ v1, x.1 = (v1, #true)%V) pvs.
   
-  Global Instance is_updating_dec : ∀ pvs, Decision (is_updating pvs).
-  Proof.
-    intros pvs. rewrite /is_updating. apply Exists_dec. intros [x1 x2].
-    rewrite /=. destruct x1.
-    - right; intros [v1 H']; try done.
-    - right; intros [v1 H']; try done.
-    - destruct (decide (x1_2 = #true)) as [-> | Hx1]. 
-      + left. by exists x1_1.
-      + right. intros [v1 H']. inversion H'. done.
-    - right; intros [v1 H']; try done.
-    - right; intros [v1 H']; try done.
-  Qed.
-
-  Parameter dsOp_spec: ∀ N γ_t γ_r γ_m γ_ght op r (p: proph_id) pvs 
-    γ_sy t_id t0 Q,
-          main_inv N γ_t γ_r γ_m γ_ght -∗
-          □ update_helping_protocol N γ_t γ_r γ_ght -∗
+  Parameter dsOp_spec: ∀ N γ_t γ_r γ_m γ_mt γ_msy op r (p: proph_id) pvs 
+     tid t0 Q,
+          main_inv N γ_t γ_r γ_m γ_mt γ_msy  -∗
+          thread_start γ_t γ_mt tid t0 -∗
+          □ update_helping_protocol N γ_t γ_r γ_mt γ_msy -∗
+          □ update_helping_protocol2 N γ_t γ_r γ_mt γ_msy -∗
             {{{ proph p pvs ∗ 
-                (⌜is_updating pvs⌝ ∗ au N γ_r op Q ∨
-                  ⌜¬ is_updating pvs⌝ ∗ thread_vars γ_t γ_ght γ_sy t_id t0) }}} 
-                  dsOp (Op_to_val op) #r #p
-            {{{ (res: resT), RET #res; 
-                  ⌜is_updating pvs⌝ ∗ Q #res
-                ∨ ⌜¬ is_updating pvs⌝ ∗ past_lin_witness γ_m op res t0 }}}.
-
+                (match process_proph tid pvs with
+                  None => au N γ_r op Q
+                | Some (i, None) => True
+                | Some (i, Some j) => au N γ_r op Q end) }}}
+                  dsOp (Op_to_val op) #r #p @ ⊤
+            {{{ (res: resT) pvs', RET #res;
+                proph p pvs' ∗
+                (match process_proph tid pvs with
+                  None => ⌜process_proph tid pvs' = None⌝ 
+                | Some (i, None) => past_lin_witness γ_m op res t0
+                | Some (i, Some j) => Q #res ∨ 
+                    ⌜∃ i' j', process_proph tid pvs' = Some(i', Some (j'))⌝ end) }}}.
+  
 End HINDSIGHT_SPEC.
 
 Module CLIENT_SPEC (DS : DATA_STRUCTURE) (HS: HINDSIGHT_SPEC DS).
@@ -80,14 +73,15 @@ Module CLIENT_SPEC (DS : DATA_STRUCTURE) (HS: HINDSIGHT_SPEC DS).
       let: "p_upd" := NewProph in
       let: "p" := NewProph in
       let: "v" := dsOp "OP" "r" "p_upd" in
+      resolve_proph: "p_upd" to: "t_id";;
       resolve_proph: "p" to: "v";;
       "v".
 
 
-  Lemma dsOp'_spec N γ_t γ_r γ_m γ_ght op (r: loc) :
-          main_inv N γ_t γ_r γ_m γ_ght -∗
+  Lemma dsOp'_spec N γ_t γ_r γ_m γ_mt γ_msy op (r: loc) :
+          main_inv N γ_t γ_r γ_m γ_mt γ_msy -∗
               <<< ∀∀ a, dsRep γ_r a >>> 
-                     dsOp' (Op_to_val op) #r @ ↑(cntrN N) ∪ ↑(threadN N)
+                     dsOp' (Op_to_val op) #r @ ↑N
               <<< ∃∃ a' res, dsRep γ_r a' ∗ ⌜seq_spec op a a' res⌝, 
                   RET #res >>>.
   Proof.
@@ -100,13 +94,14 @@ Module CLIENT_SPEC (DS : DATA_STRUCTURE) (HS: HINDSIGHT_SPEC DS).
     wp_apply (typed_proph_wp_new_proph1 resTTypedProph); first done.
     iIntros (vp p2) "Hproph2". wp_pures.
     
-    iAssert (update_helping_protocol N γ_t γ_r γ_ght)%I 
+    iAssert (update_helping_protocol N γ_t γ_r γ_mt γ_msy)%I 
         as "Upd_help". 
     { iIntros (M T s)"%Dom_M Ds Prot".
-      iDestruct "Prot" as (R G)"(HG & Domm_G & Hstar)".
+      iDestruct "Prot" as (Mt Msy)"(HMt & HMsy & %Domm_Mt & Hstar_t & Hstar_sy)".
+      set R := dom Msy.
       iAssert (dsRep γ_r (abs s) -∗
-        ([∗ set] t_id ∈ R, Reg N γ_t γ_r γ_ght t_id M) ={⊤ ∖ ↑cntrN N}=∗
-        (([∗ set] t_id ∈ R, Reg N γ_t γ_r γ_ght t_id (<[T+1:=s]> M))
+        ([∗ set] t_id ∈ R, Reg N γ_t γ_r γ_mt γ_msy t_id M) ={⊤ ∖ ↑cntrN N}=∗
+        (([∗ set] t_id ∈ R, Reg N γ_t γ_r γ_mt γ_msy t_id (<[T+1:=s]> M))
         ∗ dsRep γ_r (abs s)))%I as "H'".
       { iIntros "Ds". 
         iInduction R as [|tid' R' tid_notin_R IH] "HInd" using set_ind_L; 
@@ -116,8 +111,8 @@ Module CLIENT_SPEC (DS : DATA_STRUCTURE) (HS: HINDSIGHT_SPEC DS).
         assert (({[tid']} ∪ R') ∖ {[tid']} = R') as HR'. set_solver. rewrite HR'.
         iIntros "(Htid & Hbigstar)". 
         iMod ("HInd" with "[$Ds] Hbigstar") as "(H' & Ds)". iFrame "H'". 
-        iDestruct "Htid" as (γ_tk' γ_sy' Q' op' vp' t0' vtid')
-          "(Hproph & #Hthd & Hsy & #HthInv)".
+        iDestruct "Htid" as (γ_tk' γ_sy' Q' op' vp' t0')
+          "(#Hthst & #Hthsy & Hsy & #HthInv)".
         iInv "HthInv" as (M'' T'')"Hstate".
         iDestruct "Hstate" as "(>Hsy' & >%Dom_M'' & >%Ht0 & Hstate)".
         iAssert (⌜M'' = M⌝)%I as %->.
@@ -162,7 +157,7 @@ Module CLIENT_SPEC (DS : DATA_STRUCTURE) (HS: HINDSIGHT_SPEC DS).
             iModIntro. iSplitL "Hsy HΦ". iNext. iExists (<[T+1:=s]> M), (T+1).
             iFrame "∗%". iRight. iSplitL; last first. iPureIntro. exists (T+1). 
             split. split; try done. by rewrite lookup_total_insert. by iLeft.
-            iModIntro. iFrame. iExists γ_tk', γ_sy', Q', op', vp', t0', vtid'.
+            iModIntro. iFrame. iExists γ_tk', γ_sy', Q', op', vp', t0'.
             iFrame "∗#%".
           + iModIntro. iSplitL "AU Hc Hsy". iNext. iExists (<[T+1:=s]> M), (T+1).
             iFrame "∗%". iLeft. iFrame. iPureIntro. 
@@ -170,41 +165,155 @@ Module CLIENT_SPEC (DS : DATA_STRUCTURE) (HS: HINDSIGHT_SPEC DS).
               rewrite lookup_total_insert in Ht2. done.
               apply Past_W. exists t. split. lia. 
               rewrite lookup_total_insert_ne in Ht2; try done. } 
-            iModIntro. iFrame. iExists γ_tk', γ_sy', Q', op', vp', t0', vtid'.
+            iModIntro. iFrame. iExists γ_tk', γ_sy', Q', op', vp', t0'.
             iFrame "∗#%".
         - iDestruct "HDone" as "(HDone & >%PastW)".
           iModIntro. iSplitL "HDone Hsy". iNext. iExists (<[T+1:=s]> M), (T+1).
           iFrame "∗%". iRight. iSplitL; last first. iPureIntro.
           { destruct PastW as [t [Ht1 Ht2]]. exists t. split. lia.
             rewrite lookup_total_insert_ne. done. lia. } iFrame.
-          iModIntro. iFrame. iExists γ_tk', γ_sy', Q', op', vp', t0', vtid'.
+          iModIntro. iFrame. iExists γ_tk', γ_sy', Q', op', vp', t0'.
           iFrame "∗#%". }
-      iPoseProof ("H'" with "[$Ds] [$Hstar]") as ">(Hstar & Ds)".
-      iModIntro. iFrame. iExists R, G. iFrame. }
+      iPoseProof ("H'" with "[$Ds] [$Hstar_sy]") as ">(Hstar_sy & Ds)".
+      iModIntro. iFrame. iExists Mt, Msy. iFrame "∗%". }
+
+    iAssert (update_helping_protocol2 N γ_t γ_r γ_mt γ_msy)%I 
+        as "Upd_help2". 
+    { iIntros (M T s')"%Dom_M %Habs Prot".
+      iDestruct "Prot" as (Mt Msy)"(HMt & HMsy & %Domm_Mt & Hstar_t & Hstar_sy)".
+      set R := dom Msy.
+      iAssert (([∗ set] t_id ∈ R, Reg N γ_t γ_r γ_mt γ_msy t_id M) ={⊤ ∖ ↑cntrN N}=∗
+        (([∗ set] t_id ∈ R, Reg N γ_t γ_r γ_mt γ_msy t_id (<[T+1:=s']> M))))%I as "H'".
+      { iInduction R as [|tid' R' tid_notin_R IH] "HInd" using set_ind_L; 
+          auto using big_sepS_empty'.
+        rewrite (big_sepS_delete _ ({[tid']} ∪ R') tid'); last by set_solver.
+        rewrite (big_sepS_delete _ ({[tid']} ∪ R') tid'); last by set_solver.
+        assert (({[tid']} ∪ R') ∖ {[tid']} = R') as HR'. set_solver. rewrite HR'.
+        iIntros "(Htid & Hbigstar)". 
+        iMod ("HInd" with "Hbigstar") as "H'". iFrame "H'". 
+        iDestruct "Htid" as (γ_tk' γ_sy' Q' op' vp' t0')
+          "(#Hthst & #Hthsy & Hsy & #HthInv)".
+        iInv "HthInv" as (M'' T'')"Hstate".
+        iDestruct "Hstate" as "(>Hsy' & >%Dom_M'' & >%Ht0 & Hstate)".
+        iAssert (⌜M'' = M⌝)%I as %->.
+        { iPoseProof (own_valid_2 _ _ _ with "[$Hsy] [$Hsy']") as "%H'".
+          rewrite frac_agree_op_valid_L in H'. iPureIntro; symmetry; apply H'. }
+        assert (T'' = T) as ->.
+        { rewrite Dom_M in Dom_M''. apply gset_seq_eq in Dom_M''. done. }
+        iAssert (|={⊤ ∖ ↑cntrN N ∖ ↑threadN N}=> 
+            own γ_sy' (to_frac_agree (1 / 2) (<[T+1:=s']> M))
+          ∗ own γ_sy' (to_frac_agree (1 / 2) (<[T+1:=s']> M)))%I
+          with "[Hsy Hsy']" as ">(Hsy & Hsy')".
+        { iCombine "Hsy Hsy'" as "H'". 
+          iEval (rewrite <-frac_agree_op) in "H'".
+          iEval (rewrite Qp.half_half) in "H'".
+          iMod ((own_update (γ_sy') (to_frac_agree 1 M) 
+                        (to_frac_agree 1 (<[T+1 := s']> M))) with "[$H']") as "H'".
+          { apply cmra_update_exclusive. 
+            rewrite /valid /cmra_valid /= /prod_valid_instance.
+            split; simpl; try done. }
+          iEval (rewrite <-Qp.half_half) in "H'".
+          iEval (rewrite frac_agree_op) in "H'".  
+          iDestruct "H'" as "(Hsy & Hsy')". by iFrame. }
+        assert (dom (<[(T + 1)%nat:=s']> M) = gset_seq 0 (T + 1)) as Dom_M'.
+        { rewrite dom_insert_L Dom_M. apply set_eq_subseteq. split.
+          all: intros x; rewrite elem_of_union elem_of_singleton 
+            !elem_of_gset_seq; lia. }
+        assert (t0' ≤ T+1) as Ht0' by lia.
+        iDestruct "Hstate" as "[HPending | HDone]".
+        - iDestruct "HPending" as "(AU & >Hc & >%Past_W)".
+          iModIntro. iSplitL "AU Hc Hsy". iNext. iExists (<[T+1:=s']> M), (T+1).
+          iFrame "∗%". iLeft. iFrame. iPureIntro. 
+          { intros [t [Ht1 Ht2]]. destruct (decide (t = T+1)) as [-> | Ht].
+            rewrite lookup_total_insert Habs in Ht2. 
+            apply Past_W. exists T. split. lia. done.
+            rewrite lookup_total_insert_ne in Ht2; try done.
+            apply Past_W. exists t. split. lia. done. } 
+          iModIntro. iFrame. iExists γ_tk', γ_sy', Q', op', vp', t0'.
+          iFrame "∗#%".
+        - iDestruct "HDone" as "(HDone & >%PastW)".
+          iModIntro. iSplitL "HDone Hsy". iNext. iExists (<[T+1:=s']> M), (T+1).
+          iFrame "∗%". iRight. iSplitL; last first. iPureIntro.
+          { destruct PastW as [t [Ht1 Ht2]]. exists t. split. lia.
+            rewrite lookup_total_insert_ne. done. lia. } iFrame.
+          iModIntro. iFrame. iExists γ_tk', γ_sy', Q', op', vp', t0'.
+          iFrame "∗#%". }
+      iPoseProof ("H'" with "[$Hstar_sy]") as ">Hstar_sy".
+      iModIntro. iFrame. iExists Mt, Msy. iFrame "∗%". }
+
+    iApply fupd_wp. 
+    iInv "HInv" as (M0 T0 s0) "(Ds & >%Habs0 & Hist & Help & Templ)".
+    iApply (lc_fupd_add_later with "Hc"). iNext. 
+    iDestruct "Help" as (Mt0 Msy0)"(HMt & HMsy & %Domm_Mt0 & Hstar_t & Hstar_sy)".
+  
+    iAssert (¬ ⌜tid ∈ dom Mt0⌝)%I as %tid_notin_Mt0.
+    { iIntros "%H'". 
+      iEval (rewrite (big_sepS_elem_of_acc _ (dom Mt0) tid); 
+        last by eauto) in "Hstar_t".
+      iDestruct "Hstar_t" as "(H' & _)". iDestruct "H'" as (?)"H'".
+      iApply (proph1_exclusive tid with "[Htid]"); try done. }
     
-    destruct (decide (is_updating pvs)) as [Hpvs | Hpvs].
-    - wp_apply (dsOp_spec with "[] [] [AU Hproph1]"); try done.
-      { iFrame "Hproph1". iLeft. iFrame "AU %". }
-      iIntros (res)"Hor". iDestruct "Hor" as "[Hor | Hor]"; last first.
-      { iDestruct "Hor" as "(% & _)". exfalso; try done. }
-      iDestruct "Hor" as "(_&HΦ)". wp_pures. 
+    iPoseProof (own_update _ (● Mt0) 
+      (● (<[tid := to_agree T0]> Mt0) ⋅ ◯ {[tid := to_agree T0]}) with "HMt")
+      as ">(HMt & Thd_st')".
+    { apply auth_update_alloc, alloc_local_update; last done.
+      apply not_elem_of_dom. done. }
+    
+    iDestruct "Hist" as (M0')"(H'&H'')".
+    iPoseProof (own_update _ (● MaxNat T0) (● MaxNat T0 ⋅ ◯ MaxNat T0) 
+      with "H'") as ">(H' & Thd_st'')".
+    { apply (auth_update_alloc _ _ (MaxNat T0)), max_nat_local_update. lia. }
+    iAssert (hist γ_t γ_m M0 T0) with "[H' H'']" as "Hist".
+    { iExists M0'. iFrame. } clear M0'.
+    iAssert (thread_start γ_t γ_mt tid T0) with "[Thd_st'' Thd_st']" as "#Thd_st".
+    { iFrame. } iClear "Thd_st' Thd_st''".
+
+    set pres := process_proph tid pvs.
+    assert (process_proph tid pvs = pres) as Def_pres by done.
+    destruct pres as [[i o] | ]; last first; last (destruct o as [j |]).
+
+    - iModIntro. iSplitR "AU Hproph1 Hproph2". iNext. 
+      iExists M0, T0, s0. iFrame "∗%".
+      iExists (<[tid := to_agree T0]> Mt0), Msy0. iFrame. iSplitR. iPureIntro.
+      rewrite dom_insert_L. clear -Domm_Mt0; set_solver. rewrite dom_insert_L.
+      rewrite big_sepS_union. iFrame. rewrite big_sepS_singleton. by iExists vtid.
+      set_solver. iModIntro.
+
+      wp_apply (dsOp_spec with "[] [] [] [] [AU Hproph1]"); try done.
+      { iFrame "Hproph1". rewrite Def_pres. iFrame "AU". }
+      iIntros (res pvs')"(Hproph1 & Hmatch)". rewrite Def_pres. wp_pures.
+      iDestruct "Hmatch" as %Hpvs'. 
+      wp_apply (wp_resolve_proph with "[Hproph1]"); try done.
+      iIntros (pvs'')"(%Def_pvs' & Hproph1)". exfalso. 
+      apply process_proph_case1 in Hpvs'. rewrite Forall_lookup in Hpvs'.
+      assert (pvs' !! 0 = Some (#(), #tid)) as H'. rewrite Def_pvs'. set_solver.
+      pose proof Hpvs' 0 _ H' as H''. by simpl in H''.
+    
+    - iModIntro. iSplitR "AU Hproph1 Hproph2". iNext. 
+      iExists M0, T0, s0. iFrame "∗%".
+      iExists (<[tid := to_agree T0]> Mt0), Msy0. iFrame. iSplitR. iPureIntro.
+      rewrite dom_insert_L. clear -Domm_Mt0; set_solver. rewrite dom_insert_L.
+      rewrite big_sepS_union. iFrame. rewrite big_sepS_singleton. by iExists vtid.
+      set_solver. iModIntro.
+
+      wp_apply (dsOp_spec with "[] [] [] [] [AU Hproph1]"); try done.
+      { iFrame "Hproph1". rewrite Def_pres. iFrame "AU". }
+      iIntros (res pvs')"(Hproph1 & Hmatch)". rewrite Def_pres. wp_pures.
+      wp_apply (wp_resolve_proph with "[Hproph1]"); try done.
+      iIntros (pvs'')"(%Def_pvs' & Hproph1)". wp_pures.
+      iDestruct "Hmatch" as "[HΦ | %H']"; last first.
+      { exfalso. destruct H' as [i' [j' H']].
+        assert (pvs' !! 0 = Some (#(), #tid)) as Hp0. rewrite Def_pvs'; set_solver.
+        apply process_proph_case3 in H'. destruct H' as (Hi'&Hj'&Hji'&_).
+        destruct (decide (i' = 0)) as [-> | Hi0]; try (done || lia).
+        apply list_lookup_total_correct in Hp0. assert (0 < i') as H'' by lia.
+        pose proof Hj' 0 H'' as H1'. rewrite Hp0 in H1'. done. }
+      
       wp_apply (typed_proph_wp_resolve1 resTTypedProph with "Hproph2"); try done.
       { rewrite /typed_proph_from_val /=. by rewrite resT_proph_resolve. }
       wp_pures. iModIntro. iIntros "_". wp_pures. done.
-    - iApply fupd_wp. 
-      iInv "HInv" as (M0 T0 s0) "(Ds & >%Habs0 & Hist & Help & Templ)".
-      iApply (lc_fupd_add_later with "Hc"). iNext. 
-      iDestruct "Help" as (R0 G0)"(HG & %Domm_G0 & Hstar)".
-      
-      iAssert (¬ ⌜tid ∈ R0⌝)%I as %tid_notin_R0.
-      { iIntros "%H'". 
-        iEval (rewrite (big_sepS_elem_of_acc _ (R0) tid); 
-          last by eauto) in "Hstar".
-        iDestruct "Hstar" as "(H' & _)".
-        iDestruct "H'" as (? ? ? ? ? ? ?)"(H' & _)".
-        iApply (proph1_exclusive tid with "[Htid]"); try done. }
-            
-      iMod (own_alloc (to_frac_agree (1) (M0))) 
+    
+    - iMod (own_alloc (to_frac_agree (1) (M0))) 
               as (γ_sy)"Hfr_t". { try done. }        
       iEval (rewrite <-Qp.half_half) in "Hfr_t".      
       iEval (rewrite (frac_agree_op (1/2) (1/2) _)) in "Hfr_t". 
@@ -212,25 +321,15 @@ Module CLIENT_SPEC (DS : DATA_STRUCTURE) (HS: HINDSIGHT_SPEC DS).
 
       iMod (own_alloc (Excl ())) as (γ_tk) "Token"; first try done.
 
-      set (<[ tid := to_agree (T0, γ_sy) ]> G0) as G0'.
-      iDestruct (own_update _ _ 
-        (● G0' ⋅ ◯ {[ tid := to_agree (T0, γ_sy) ]})
-               with "HG") as ">HG".
-      { apply auth_update_alloc. rewrite /G0'.
-        apply alloc_local_update; last done. apply not_elem_of_dom.
-        by rewrite Domm_G0 in tid_notin_R0. }
-      iDestruct "HG" as "(HG & #Hreg_gh)".
+      iPoseProof (own_update _ (● Msy0) 
+        (● (<[tid := to_agree γ_sy]> Msy0) ⋅ ◯ {[tid := to_agree γ_sy]}) 
+        with "HMsy") as ">(HMsy & #Thd_sy)".
+      { apply auth_update_alloc, alloc_local_update; last done.
+        apply not_elem_of_dom. clear -tid_notin_Mt0 Domm_Mt0. set_solver. }
 
       iAssert (⌜dom M0 = gset_seq 0 T0⌝)%I as %Dom_M0. 
       { by iDestruct "Hist" as (M0') "(_&_&%&_)". }
-      iDestruct "Hist" as (M0')"(H'&H'')".
-      iDestruct (own_update _ _ (● (MaxNat T0) ⋅ ◯ (MaxNat T0)) with "H'") 
-        as ">H1'".
-      { apply auth_update_alloc. apply max_nat_local_update. try done. }
-      iDestruct "H1'" as "(H' & #HfragT0)".
-      iAssert (hist γ_t γ_m M0 T0) with "[H' H'']" as "Hist".
-      { iExists M0'; iFrame. }
-      
+
       iAssert (|={⊤ ∖ ↑cntrN N}=> dsRepI γ_r (abs s0) ∗ 
         (inv (threadN N) (∃ M T, State γ_sy γ_tk (au N γ_r op Φ) Φ M T op vp T0)))%I
         with "[Ds AU Hc' Hreg_sy1]" as "H'".
@@ -267,26 +366,20 @@ Module CLIENT_SPEC (DS : DATA_STRUCTURE) (HS: HINDSIGHT_SPEC DS).
 
       iModIntro. iSplitR "Hproph1 Hproph2 Token". iNext.
       iExists M0, T0, s0. iFrame "∗%".
-      iExists (R0 ∪ {[tid]}), G0'. iFrame.
-      iSplitR. iPureIntro. subst G0'. rewrite dom_insert_L.
-      clear -Domm_G0; set_solver.
-      rewrite (big_sepS_delete _ (R0 ∪ {[tid]}) tid); last by set_solver.
-      iSplitR "Hstar". 
-      iExists γ_tk, γ_sy, Φ, op, vp, T0, vtid. iFrame "∗#".
-      assert ((R0 ∪ {[tid]}) ∖ {[tid]} = R0) as H' 
-                by (clear -tid_notin_R0; set_solver).
-      by rewrite H'.
+      iExists (<[tid:=to_agree T0]> Mt0), (<[tid:=to_agree γ_sy]> Msy0). iFrame.
+      iSplitR. iPureIntro. rewrite !dom_insert_L. clear -Domm_Mt0; set_solver.
+      rewrite !dom_insert_L. rewrite !big_sepS_union. rewrite !big_sepS_singleton.
+      iFrame. iSplitL "Htid". by iExists vtid.
+      iExists γ_tk, γ_sy, Φ, op, vp, T0. iFrame "∗#". set_solver. set_solver.
       
-      iAssert (thread_vars γ_t γ_ght γ_sy tid T0)%I as "#Thd".
-      { iFrame "#". }
-    
-      iModIntro. wp_apply (dsOp_spec with "[] [] [Hproph1]"); try done.
-      { iFrame "Hproph1". iRight. iFrame "#%". }
+      iModIntro. wp_apply (dsOp_spec with "[] [] [] [] [Hproph1]"); try done.
+      { iFrame "Hproph1". by rewrite Def_pres. }
+
+      iIntros (res pvs')"(Hproph1 & Hmatch)". rewrite Def_pres. wp_pures.
+      wp_apply (wp_resolve_proph with "[Hproph1]"); try done.
+      iIntros (pvs'')"(%Def_pvs' & Hproph1)". wp_pures.
       
-      iIntros (res)"Hor". iDestruct "Hor" as "[Hor | Hor]".
-      { iDestruct "Hor" as "(%&_)"; exfalso; try done. }
-      
-      iDestruct "Hor" as "(_&#PastW)". wp_pures. 
+      iDestruct "Hmatch" as "#PastW". wp_pures. 
       wp_apply ((typed_proph_wp_resolve1 resTTypedProph 
                 _ _ _ _ _ _ _ (res))
         with "Hproph2"); try done.
@@ -296,12 +389,12 @@ Module CLIENT_SPEC (DS : DATA_STRUCTURE) (HS: HINDSIGHT_SPEC DS).
       wp_pure credit: "Hc2". 
       iInv "HInv" as (M1 T1 s1) "(>Ds & >%Habs1 & >Hist & Help & Templ)".
       iApply (lc_fupd_add_later with "Hc1"). iNext. 
-      iDestruct "Help" as (R1 G1)"(HG & %Domm_G1 & Hstar)".
+      iDestruct "Help" as (Mt1 Msy1)"(HMt & HMsy & %Domm_Mt1 & Hstar_t & Hstar_sy)".
       
-      iAssert (⌜tid ∈ R1⌝)%I as "%tid_in_R1".
-      { iPoseProof (own_valid_2 _ _ _ with "[$HG] [$Hreg_gh]") as "%H'".
+      iAssert (⌜tid ∈ dom Msy1⌝)%I as "%tid_in_Msy1".
+      { iPoseProof (own_valid_2 _ _ _ with "[$HMsy] [$Thd_sy]") as "%H'".
         apply auth_both_valid_discrete in H'. destruct H' as [H' _].
-        apply dom_included in H'. rewrite dom_singleton_L -Domm_G1 in H'.
+        apply dom_included in H'. rewrite dom_singleton_L in H'.
         iPureIntro. clear -H'; set_solver. }
     
       iAssert (⌜dom M1 = gset_seq 0 T1⌝)%I as %Dom_M1. 
@@ -310,12 +403,11 @@ Module CLIENT_SPEC (DS : DATA_STRUCTURE) (HS: HINDSIGHT_SPEC DS).
       iInv "HthInv" as (M1_th T1_th)"(>Hth_sy & >%Dom_M1' & >%Ht0 & Hth_or)".
       iApply (lc_fupd_add_later with "Hc2"). iNext. 
       iAssert (⌜M1_th = M1⌝)%I as %->.
-      { rewrite (big_sepS_delete _ R1 tid); try done.
-        iDestruct "Hstar" as "(H' & _)". 
-        iDestruct "H'" as (? γ_sy' ?????)"(_&#H'&H''&_)".
-        iDestruct "Thd" as "(H1'&_)". iDestruct "H'" as "(H1''&_)".
-        iCombine "H1'" "H1''" as "H2'".
-        iPoseProof (own_valid with "H2'") as "%HV".
+      { rewrite (big_sepS_delete _ (dom Msy1) tid); try done.
+        iDestruct "Hstar_sy" as "(H' & _)". 
+        iDestruct "H'" as (? γ_sy' ????)"(_&#H'&H''&_)".
+        iCombine "H'" "Thd_sy" as "H1'".
+        iPoseProof (own_valid with "H1'") as "%HV".
         rewrite auth_frag_valid in HV. 
         apply singleton_valid, to_agree_op_inv, leibniz_equiv in HV. 
         inversion HV. subst γ_sy'.
@@ -342,8 +434,7 @@ Module CLIENT_SPEC (DS : DATA_STRUCTURE) (HS: HINDSIGHT_SPEC DS).
       iModIntro. iSplitL "Hth_sy Token".
       iNext. iExists M1, T1. iFrame "Hth_sy %". iRight. iFrame "#". by iRight.
       iModIntro. iSplitR "HΦ". iNext. iExists M1, T1, s1; iFrame "∗%".
-      iExists R1, G1; iFrame "∗%".
-      done. Unshelve. all: try done. admit.
-  Admitted.
+      iExists Mt1, Msy1; iFrame "∗%". done. Unshelve. done.
+  Qed.
   
 End CLIENT_SPEC.
